theories/unification.v
@@ -4,6 +4,55 @@ Import ListNotations.
 
 (** * Verified Unification Algorithm *)
 
+(** ** Finite substitutions and replacements *)
+
+Definition fin_subst := @fin_map pattern.
+
+Definition interp (f : fin_subst ) : psubstitution :=
+  fun x => match get f x with Some vx => vx | None => Pvar x end.
+
+Definition replace (p : pattern) (x : nat) (q : pattern) :=
+  psubst p (interp [(x, q)]).
+
+Notation "p '⟨' x ':=' q '⟩'" := (replace p x q) (at level 60).
+Notation "p '.⟨' s '⟩'" := (psubst p s) (at level 60).
+
+(** Replacement in a list of equations of the forme [term = term] *)
+Definition replace_all_1 (l : list (pattern * pattern)) (x : nat) (p : pattern) :=
+  map (fun '(p1, p2) => (p1⟨x := p⟩, p2⟨x := p⟩)) l.
+
+(** Replacement in a list of equations of the form [var = term].
+    Only the right hand sides are modified.
+*)
+Definition replace_all_2 (l : list (nat * pattern)) (x : nat) (p : pattern) :=
+  map (fun '(y, py) => (y, py⟨x := p⟩)) l.
+
+(** ** Unifiers *)
+
+(** What it means that a substitution unifies 2 patterns *)
+Definition unifier u p1 p2 : Prop :=
+  p1.⟨u⟩ = p2.⟨u⟩.
+
+(** What it means to be a solution to a set of equations *)
+Definition satisfy (u : psubstitution) equs :=
+  Forall (fun '(x, y) => unifier u x y) equs.
+
+Lemma unifier_cons:
+  forall u f1 pat1 pats1 f2 pat2 pats2,
+    unifier u (Pcmp f1 (pat1::pats1)) (Pcmp f2 (pat2::pats2)) <->
+    (unifier u pat1 pat2 /\ unifier u (Pcmp f1 pats1) (Pcmp f2 pats2)).
+Proof.
+  intros. split.
+  - intros H. inversion H; subst.
+    unfold unifier. split; simpl; auto.
+    now rewrite H3.
+  - intros [H1 H2].
+    unfold unifier in *. simpl.
+    rewrite H1. now injection H2 as -> ->.
+Qed.
+
+(** ** Algorithm *)
+
 (** As for matching, a state of the algorithm is a list of equations to be solved and a current solution.
     The only difference is that unification equations are of the form [(pattern, pattern)]
     Solutions are represented as finite maps from variables to patterns ([pattern])
@@ -12,3 +61,133 @@ Record state := {
   equations : list (pattern * pattern);
   solution  : @fin_map pattern;
 }.
+
+(** At every iteration, the algorithm either fails, update the current state,
+    or terminates with a solution *)
+Inductive status :=
+  | Failure
+  | Update (st : state)
+  | Success (sub : @fin_map pattern).
+
+(** What it means for to set of equations to be equivalent *)
+Definition equiv (equs1 equs2 : list (pattern * pattern)) :=
+  forall u, satisfy u equs1 <-> satisfy u equs2.
+
+(** Intepreting a finite map as a set of equations *)
+Definition map_as_equations (m : @fin_map pattern) :=
+  map (fun '(x, y) => (Pvar x, y)) m.
+
+(** Intepreting a state as set of equations *)
+Definition state_as_equations (st : state) :=
+  equations st ++ map_as_equations (solution st).
+
+Definition state_equiv (st1 st2 : state) :=
+  equiv (state_as_equations st1) (state_as_equations st2).
+
+(** Decompose the problem of unifying two vectors
+    into a list of equations.
+    The generated equations are collected on top
+    of a provided accumulator.
+*)
+Fixpoint decompose (l1 : list pattern) (l2 : list pattern) :=
+  match l1, l2 with
+  | [], [] => Some []
+  | x::xs, y::ys =>
+    do equs <- decompose xs ys;
+    Some ((x, y)::equs)
+  | _, _ => None
+  end.
+
+Definition unification_step (st : state) :=
+  match equations st with
+  | [] => Success (solution st)
+  | (t1, t2)::xs =>
+    match t1, t2 with
+    | Pcmp f1 l1, Pcmp f2 l2 =>
+      if (f1 =? f2)%string then
+        match decompose l1 l2 with
+        | Some equs => Update (Build_state (equs ++ xs) (solution st))
+        | None => Failure
+        end
+      else Failure
+    | Pvar n, t | t, Pvar n =>
+      if is_free t n then
+        Failure
+      else
+        Update (Build_state (replace_all_1 xs n t) ((n, t)::(replace_all_2 (solution st) n t)))
+    end
+  end.
+
+Lemma decompose_equiv:
+  forall s1 s2 l1 l2 l,
+    (s1 =? s2)%string = true ->
+    decompose l1 l2 = Some l ->
+    equiv l [(Pcmp s1 l1, Pcmp s2 l2)].
+Proof.
+  intros * ->%String.eqb_eq Hdec sub.
+  induction l2 in l, l1, Hdec, sub |-*.
+  - destruct l1; try easy.
+    inversion_clear Hdec.
+    repeat econstructor.
+  - destruct l1; simpl in *; try easy.
+    destruct (decompose l1 l2) as [l'|] eqn:Heq; simpl in *; try easy.
+    inversion Hdec; subst. clear Hdec.
+    specialize (IHl2 _ _ Heq sub) as [H1 H2].
+    split; intros.
+    + inversion_clear H as [| ? ? H3 H4].
+      specialize (H1 H4).
+      inversion_clear H1 as [| ? ? H5 _].
+      repeat econstructor.
+      apply unifier_cons.
+      now repeat econstructor.
+    + inversion H as [| ? ? H3 _]; subst.
+      apply unifier_cons in H3 as [H3 H4].
+      econstructor; auto.
+      apply H2. now repeat econstructor.
+Qed.
+
+Theorem unification_step_equiv:
+  forall st1 st2,
+    unification_step st1 = Update st2 ->
+    state_equiv st1 st2.
+Proof.
+  intros [equs1 sol1] [equs2 sol2] Hstep sub.
+  induction equs1 as [| [dat1 pat1] equs1 _] in equs2, sol2, Hstep |-*; try easy.
+  destruct dat1, pat1; try easy.
+  cbn in Hstep.
+  destruct (s =? s0)%string eqn:Heq1; try easy.
+  destruct (decompose l l0) eqn:Heq2; try easy.
+  apply String.eqb_eq in Heq1; subst.
+  inversion Hstep; subst. clear Hstep.
+  apply (decompose_equiv s0 s0 _ _ _ (String.eqb_refl s0)) in Heq2.
+  specialize (Heq2 sub).
+  unfold state_as_equations. simpl. split.
+  - intros H. inversion H as [|? ? H2 H3]; subst.
+    clear H. apply Forall_app in H3 as [H3 H4].
+    do 2 (apply Forall_app; split; auto).
+    apply Heq2. now econstructor.
+  - intros [[H1 H2]%Forall_app H3]%Forall_app.
+    apply Forall_cons.
+    + apply Heq2 in H1. now inversion H1.
+    + apply Forall_app; split; auto.
+Qed.
+
+(** ** INVARIAAAAAANT !!!! *)
+
+(** For all binding [x = vx] in the current solution,
+    [x] is does not occur in [vx] and in the remaning
+    equations.
+*)
+Definition invariant (st : state) :=
+  forall x vx, In (x, vx) (solution st) ->
+    ~(free_var vx x) /\
+    forall pat1 pat2, In (pat1, pat2) (equations st) ->
+      ~free_var pat1 x /\ ~free_var pat2 x.
+
+Lemma unification_step_invariant:
+  forall st1 st2,
+    invariant st1 ->
+    unification_step st1 = Update st2 ->
+    invariant st2.
+Proof.
+Admitted.
